src/progress.lean
@@ -1,12 +1,8 @@
 import .definitions3 .logic
 
-@[reducible]
-def is_value(s: stack): Prop :=
-  ∃(R: spec) (σ: env) (x: var) (v: value), s = (R, σ, exp.return x) ∧ (σ x = v)
-
 lemma exp.progress {R: spec} {P: prop} {Q: propctx} {e: exp} {σ: env}:
       (⊩ σ: P) → (FV R.to_prop ⊆ FV P) → (σ ⊨ R.to_prop.to_vc) → (R ⋀ P ⊩ e: Q) → 
-      is_value (R, σ, e) ∨ ∃s', (R, σ, e) ⟶ s' :=
+      is_dvalue (R, σ, e) ∨ ∃s', (R, σ, e) ⟹ s' :=
   assume env_verified: (⊩ σ : P),
   assume fv_R: FV R.to_prop ⊆ FV P,
   assume R_valid: (σ ⊨ R.to_prop.to_vc),
@@ -17,34 +13,34 @@ lemma exp.progress {R: spec} {P: prop} {Q: propctx} {e: exp} {σ: env}:
     have z ∈ FV P, from set.mem_of_subset_of_mem fv_R this,
     show z ∈ σ.dom, from (free_iff_contains env_verified).symm ▸ this
   ),
-  show is_value (R, σ, e) ∨ ∃s', (R, σ, e) ⟶ s', by begin
+  show is_dvalue (R, σ, e) ∨ ∃s', (R, σ, e) ⟹ s', by begin
     cases e_verified,
     case exp.dvcgen.tru x e' { from
-      let s: stack := (R, σ, lett x = true in e') in
-      have s ⟶ (R, σ[x↦value.true], e'), from step.tru,
-      have ∃s', s ⟶ s', from exists.intro (R, σ[x↦value.true], e') this,
-      show is_value s ∨ ∃s', s ⟶ s', from or.inr this
+      let s: dstack := (R, σ, lett x = true in e') in
+      have s ⟹ (R, σ[x↦value.true], e'), from dstep.tru,
+      have ∃s', s ⟹ s', from exists.intro (R, σ[x↦value.true], e') this,
+      show is_dvalue s ∨ ∃s', s ⟹ s', from or.inr this
     },
     case exp.dvcgen.fals x e' { from
-      let s: stack := (R, σ, letf x = false in e') in
-      have s ⟶ (R, σ[x↦value.false], e'), from step.fals,
-      have ∃s', s ⟶ s', from exists.intro (R, σ[x↦value.false], e') this,
-      show is_value s ∨ ∃s', s ⟶ s', from or.inr this
+      let s: dstack := (R, σ, letf x = false in e') in
+      have s ⟹ (R, σ[x↦value.false], e'), from dstep.fals,
+      have ∃s', s ⟹ s', from exists.intro (R, σ[x↦value.false], e') this,
+      show is_dvalue s ∨ ∃s', s ⟹ s', from or.inr this
     },
     case exp.dvcgen.num x n e' { from
-      let s: stack := (R, σ, letn x = n in e') in
-      have s ⟶ (R, σ[x↦value.num n], e'), from step.num,
-      have ∃s', s ⟶ s', from exists.intro (R, σ[x↦value.num n], e') this,
-      show is_value s ∨ ∃s', s ⟶ s', from or.inr this
+      let s: dstack := (R, σ, letn x = n in e') in
+      have s ⟹ (R, σ[x↦value.num n], e'), from dstep.num,
+      have ∃s', s ⟹ s', from exists.intro (R, σ[x↦value.num n], e') this,
+      show is_dvalue s ∨ ∃s', s ⟹ s', from or.inr this
     },
     case exp.dvcgen.func f x R' S' e₁ e₂ { from
-      let s: stack := (R, σ, letf f[x] req R' ens S' {e₁} in e₂) in
-      have s ⟶ (R, σ[f↦value.func f x R' S' e₁ σ], e₂), from step.closure,
-      have ∃s', s ⟶ s', from exists.intro (R, σ[f↦value.func f x R' S' e₁ σ], e₂) this,
-      show is_value s ∨ ∃s', s ⟶ s', from or.inr this
+      let s: dstack := (R, σ, letf f[x] req R' ens S' {e₁} in e₂) in
+      have s ⟹ (R, σ[f↦value.func f x R' S' e₁ σ], e₂), from dstep.closure,
+      have ∃s', s ⟹ s', from exists.intro (R, σ[f↦value.func f x R' S' e₁ σ], e₂) this,
+      show is_dvalue s ∨ ∃s', s ⟹ s', from or.inr this
     },
     case exp.dvcgen.unop op x y e' Q' x_free_in_P _ e'_verified vc_valid { from
-      let s: stack := (R, σ, letop y = op[x] in e') in
+      let s: dstack := (R, σ, letop y = op[x] in e') in
       let ⟨v, env_has_x⟩ := (val_of_free_in_pre_env env_verified fv_R x_free_in_P) in
       have closed_subst σ (prop.pre₁ op x), from (
         assume z: var,
@@ -63,12 +59,12 @@ lemma exp.progress {R: spec} {P: prop} {Q: propctx} {e: exp} {σ: env}:
       have option.is_some (unop.apply op v), from valid.pre₁.mpr this,
       have (∃v', unop.apply op v = some v'), from option.is_some_iff_exists.mp this,
       let ⟨v', op_v_is_v'⟩ := this in
-      have s ⟶ (R, σ[y↦v'], e'), from step.unop env_has_x op_v_is_v',
-      have ∃s', s ⟶ s', from exists.intro (R, σ[y↦v'], e') this,
-      show is_value s ∨ ∃s', s ⟶ s', from or.inr this
+      have s ⟹ (R, σ[y↦v'], e'), from dstep.unop env_has_x op_v_is_v',
+      have ∃s', s ⟹ s', from exists.intro (R, σ[y↦v'], e') this,
+      show is_dvalue s ∨ ∃s', s ⟹ s', from or.inr this
     },
     case exp.dvcgen.binop op x y z e' Q' x_free_in_P y_free_in_P _ e'_verified vc_valid { from
-      let s: stack := (R, σ, letop2 z = op[x,y] in e') in
+      let s: dstack := (R, σ, letop2 z = op[x,y] in e') in
       let ⟨vx, env_has_x⟩ := (val_of_free_in_pre_env env_verified fv_R x_free_in_P) in
       let ⟨vy, env_has_y⟩ := (val_of_free_in_pre_env env_verified fv_R y_free_in_P) in
       have closed_subst σ (prop.pre₂ op x y), from (
@@ -97,12 +93,12 @@ lemma exp.progress {R: spec} {P: prop} {Q: propctx} {e: exp} {σ: env}:
       have option.is_some (binop.apply op vx vy), from valid.pre₂.mpr this,
       have (∃v', binop.apply op vx vy = some v'), from option.is_some_iff_exists.mp this,
       let ⟨v', op_v_is_v'⟩ := this in
-      have s ⟶ (R, σ[z↦v'], e'), from step.binop env_has_x env_has_y op_v_is_v',
-      have ∃s', s ⟶ s', from exists.intro (R, σ[z↦v'], e') this,
-      show is_value s ∨ ∃s', s ⟶ s', from or.inr this
+      have s ⟹ (R, σ[z↦v'], e'), from dstep.binop env_has_x env_has_y op_v_is_v',
+      have ∃s', s ⟹ s', from exists.intro (R, σ[z↦v'], e') this,
+      show is_dvalue s ∨ ∃s', s ⟹ s', from or.inr this
     },
     case exp.dvcgen.app y f x e' Q' f_free_in_P x_free_in_P _ e'_verified vc_valid { from
-      let s: stack := (R, σ, letapp y = f [x] in e') in
+      let s: dstack := (R, σ, letapp y = f [x] in e') in
       let ⟨vf, env_f_is_vf⟩ := (val_of_free_in_pre_env env_verified fv_R f_free_in_P) in
       have env_has_f: f ∈ σ, from env.contains_apply_equiv.right.mp (exists.intro vf env_f_is_vf),
       let ⟨vx, env_x_is_vx⟩ := (val_of_free_in_pre_env env_verified fv_R x_free_in_P) in
@@ -161,13 +157,13 @@ lemma exp.progress {R: spec} {P: prop} {Q: propctx} {e: exp} {σ: env}:
       let ⟨g, gx, gR, gS, ge, gσ, vf_is_g⟩ := this in
       have some_vf_is_g: some vf = ↑(value.func g gx gR gS ge gσ), from some.inj.inv vf_is_g,
       have σ f = value.func g gx gR gS ge gσ, from eq.trans env_f_is_vf some_vf_is_g,
-      let s': stack := (gR, gσ[g↦value.func g gx gR gS ge gσ][gx↦vx], ge) · [R, σ, letapp y = f[x] in e'] in
-      have s ⟶ s', from step.app this env_x_is_vx,
-      have ∃s', s ⟶ s', from exists.intro s' this,
-      show is_value s ∨ ∃s', s ⟶ s', from or.inr this
+      let s': dstack := dstack.cons (gR, gσ[g↦value.func g gx gR gS ge gσ][gx↦vx], ge) R σ y f x e' in
+      have s ⟹ s', from dstep.app this env_x_is_vx,
+      have ∃s', s ⟹ s', from exists.intro s' this,
+      show is_dvalue s ∨ ∃s', s ⟹ s', from or.inr this
     },
     case exp.dvcgen.ite x e₂ e₁ Q₁ Q₂ x_free_in_P _ _ vc_valid { from
-      let s: stack := (R, σ, exp.ite x e₁ e₂) in
+      let s: dstack := (R, σ, exp.ite x e₁ e₂) in
       let ⟨v, env_has_x⟩ := (val_of_free_in_pre_env env_verified fv_R x_free_in_P) in
       have closed_subst σ (prop.term (term.unop unop.isBool x)), from (
         assume z: var,
@@ -197,63 +193,63 @@ lemma exp.progress {R: spec} {P: prop} {Q: propctx} {e: exp} {σ: env}:
         assume : v = value.true,
         have some v = some value.true, from some.inj.inv this,
         have σ x = value.true, from eq.trans env_has_x this,
-        have s ⟶ (R, σ, e₁), from step.ite_true this,
-        have ∃s', s ⟶ s', from exists.intro (R, σ, e₁) this,
-        show is_value s ∨ ∃s', s ⟶ s', from or.inr this
+        have s ⟹ (R, σ, e₁), from dstep.ite_true this,
+        have ∃s', s ⟹ s', from exists.intro (R, σ, e₁) this,
+        show is_dvalue s ∨ ∃s', s ⟹ s', from or.inr this
       ) (
         assume : v = value.false,
         have some v = some value.false, from some.inj.inv this,
         have σ x = value.false, from eq.trans env_has_x this,
-        have s ⟶ (R, σ, e₂), from step.ite_false this,
-        have ∃s', s ⟶ s', from exists.intro (R, σ, e₂) this,
-        show is_value s ∨ ∃s', s ⟶ s', from or.inr this
+        have s ⟹ (R, σ, e₂), from dstep.ite_false this,
+        have ∃s', s ⟹ s', from exists.intro (R, σ, e₂) this,
+        show is_dvalue s ∨ ∃s', s ⟹ s', from or.inr this
       )
     },
     case exp.dvcgen.return x x_free_in_P { from
-      let s: stack := (R, σ, exp.return x) in
+      let s: dstack := (R, σ, exp.return x) in
       have s_is_return: s = (R, σ, exp.return x), from rfl,
       let ⟨v, env_has_x⟩ := (val_of_free_in_pre_env env_verified fv_R x_free_in_P) in
-      have is_value_s: is_value s
+      have is_value_s: is_dvalue s
         = (∃(R': spec) (σ': env) (x': var) (v: value), s = (R', σ', exp.return x') ∧ (σ' x' = v)),
-      by unfold is_value,
+      by unfold is_dvalue,
       have (∃(R': spec) (σ': env) (x': var) (v: value), s = (R', σ', exp.return x') ∧ (σ' x' = v)),
       from exists.intro R (exists.intro σ (exists.intro x (exists.intro v ⟨s_is_return, env_has_x⟩))),
-      have is_value s, from is_value_s ▸ this,
-      show is_value s ∨ ∃s', s ⟶ s', from or.inl this
+      have is_dvalue s, from is_value_s ▸ this,
+      show is_dvalue s ∨ ∃s', s ⟹ s', from or.inl this
     }
   end
 
-theorem progress {s: stack} {Q: propctx}: (⊩ₛ s : Q) → is_value s ∨ ∃s', s ⟶ s'
+theorem progress {s: dstack} {Q: propctx}: (⊩ₛ s : Q) → is_dvalue s ∨ ∃s', s ⟹ s'
 :=
   assume s_verified: ⊩ₛ s : Q,
   begin
     induction s_verified,
     case stack.dvcgen.top σ e R P Q env_verified fv_R R_valid e_verified { from
-      show is_value (R, σ, e) ∨ ∃s', (R, σ, e) ⟶ s', from exp.progress env_verified fv_R R_valid e_verified
+      show is_dvalue (R, σ, e) ∨ ∃s', (R, σ, e) ⟹ s', from exp.progress env_verified fv_R R_valid e_verified
     },
     case stack.dvcgen.cons P P' P'' s' σ σ' f g x y fx R R' S' e₁ e₂ vₓ Q Q' Q''
                           s'_verified y_not_in_σ σ_verified σ'_verified σ''_verified fv_R R_valid g_is_func
                           x_is_v e₁_verified cont Q''_dom Q''_fv pre_vc steps ih { from
-      let s := (s' · [R, σ, letapp y = g[x] in e₁]) in
-      have s_cons: s = (s' · [R, σ, letapp y = g[x] in e₁]), from rfl,
+      let s := dstack.cons s' R σ y g x e₁ in
+      have s_cons: s = (dstack.cons s' R σ y g x e₁), from rfl,
       or.elim ih
       ( -- step return
-        assume s'_is_value: is_value s',
+        assume s'_is_value: is_dvalue s',
         let ⟨R₂, σ₂, z, v, ⟨s'_return, env2_has_z⟩⟩ := s'_is_value in
-        have s_return_cons: s = ((R₂, σ₂, exp.return z) · [R, σ, letapp y = g[x] in e₁]),
+        have s_return_cons: s = dstack.cons (R₂, σ₂, exp.return z) R σ y g x e₁,
         from s'_return ▸ s_cons,
-        have s ⟶ (R, σ[y↦v], e₁),
-        from s_return_cons.symm ▸ (step.return env2_has_z g_is_func x_is_v),
-        have ∃s', s ⟶ s',
+        have s ⟹ (R, σ[y↦v], e₁),
+        from s_return_cons.symm ▸ (dstep.return env2_has_z g_is_func x_is_v),
+        have ∃s', s ⟹ s',
         from exists.intro (R, σ[y↦v], e₁) this,
-        show is_value s ∨ ∃s', s ⟶ s', from or.inr this
+        show is_dvalue s ∨ ∃s', s ⟹ s', from or.inr this
       )
       ( -- step ctx
-        assume s'_can_step: ∃s'', s' ⟶ s'',
+        assume s'_can_step: ∃s'', s' ⟹ s'',
         let ⟨s'', s'_steps⟩ := s'_can_step in
-        have s ⟶ (s'' · [R, σ, letapp y = g[x] in e₁]), from step.ctx s'_steps,
-        have ∃s', s ⟶ s', from exists.intro (s'' · [R, σ, letapp y = g[x] in e₁]) this,
-        show is_value s ∨ ∃s', s ⟶ s', from or.inr this
+        have s ⟹ dstack.cons s'' R σ y g x e₁, from dstep.ctx s'_steps,
+        have ∃s', s ⟹ s', from exists.intro (dstack.cons s'' R σ y g x e₁) this,
+        show is_dvalue s ∨ ∃s', s ⟹ s', from or.inr this
       )
     }
   end
