src/evaluation.lean
@@ -1,6 +1,6 @@
 -- lemmas about evaluation
 
-import .definitions2
+import .definitions3
 
 -- lemmas
 
@@ -86,14 +86,14 @@ lemma binop.eq.inv {v₁ v₂: value}: binop.apply binop.eq v₁ v₂ = value.tr
     contradiction
   end
 
-lemma pre_preserved {s s': stack}: s ⟶* s' → (s.pre = s'.pre) :=
+lemma pre_preserved {s s': dstack}: s ⟹* s' → (s.pre = s'.pre) :=
   begin
     assume h1,
     induction h1,
-    case trans_step.rfl {
+    case trans_dstep.rfl {
       refl
     },
-    case trans_step.trans s₁ s₂ s₃ h2 h3 ih {
+    case trans_dstep.trans s₁ s₂ s₃ h2 h3 ih {
       apply eq.trans ih,
       cases h3,
       repeat {refl}
@@ -463,4 +463,469 @@ lemma binop_result_not_function {vx vy vz: value} {op: binop}:
 
       unfold binop.apply at h1,
       contradiction    }
+  end
+
+lemma step_dstep_progress {s s': stack}:
+      (s ⟶ s') → ∀d, stack_equiv_dstack s d → ∃d', (d ⟹ d') :=
+  begin
+    assume h1,
+
+    induction h1,
+
+    case step.tru {
+      assume d,
+      assume h2,
+      cases h2,
+
+      existsi (dstack.top R (σ[x↦value.true]) e),
+      apply dstep.tru
+    },
+
+    case step.fals {
+      assume d,
+      assume h2,
+      cases h2,
+
+      existsi (dstack.top R (σ[x↦value.false]) e),
+      apply dstep.fals
+    },
+
+    case step.num {
+      assume d,
+      assume h2,
+      cases h2,
+
+      existsi (dstack.top R (σ[x↦value.num n]) e),
+      apply dstep.num
+    },
+
+    case step.closure {
+      assume d,
+      assume h2,
+      cases h2,
+
+      existsi (dstack.top R_1 (σ[f↦value.func f x R S e₁ σ]) e₂),
+      apply dstep.closure
+    },
+
+    case step.unop {
+      assume d,
+      assume h2,
+      cases h2,
+
+      existsi (dstack.top R (σ[y↦v]) e),
+      apply dstep.unop a a_1
+    },
+
+    case step.binop {
+      assume d,
+      assume h2,
+      cases h2,
+
+      existsi (dstack.top R (σ[z↦v]) e),
+      apply dstep.binop a a_1 a_2
+    },
+
+    case step.app {
+      assume d,
+      assume h2,
+      cases h2,
+
+      existsi (dstack.cons (R, (σ'[g↦value.func g z R S e σ'][z↦v]), e) R_1 σ y f x e'),
+      apply dstep.app a a_1
+    },
+
+    case step.ite_true {
+      assume d,
+      assume h2,
+      cases h2,
+
+      existsi (dstack.top R σ e₁),
+      apply dstep.ite_true a
+    },
+
+    case step.ite_false {
+      assume d,
+      assume h2,
+      cases h2,
+
+      existsi (dstack.top R σ e₂),
+      apply dstep.ite_false a
+    },
+
+    case step.ctx s₁ s₂ σ₁ f x y e₁ steps ih {
+      assume d,
+      assume h2,
+      cases h2,
+
+      have h3, from ih d' a,
+      cases h3 with d'' h4,
+
+      existsi (dstack.cons d'' R σ₁ y f x e₁),
+      apply dstep.ctx h4
+    },
+
+    case step.return {
+      assume d,
+      assume h2,
+      cases h2,
+
+      existsi (dstack.top R_1 (σ₂[y↦v]) e'),
+      cases a_3,
+      apply dstep.return a a_1 a_2
+    }
+  end
+
+lemma step_dstep_progress.inv {d d': dstack}:
+      (d ⟹ d') → ∀s, stack_equiv_dstack s d → ∃s', (s ⟶ s') :=
+  begin
+    assume h1,
+
+    induction h1,
+
+    case dstep.tru {
+      assume s,
+      assume h2,
+      cases h2,
+
+      existsi (stack.top (σ[x↦value.true]) e),
+      apply step.tru
+    },
+
+    case dstep.fals {
+      assume s,
+      assume h2,
+      cases h2,
+
+      existsi (stack.top (σ[x↦value.false]) e),
+      apply step.fals
+    },
+
+    case dstep.num {
+      assume s,
+      assume h2,
+      cases h2,
+
+      existsi (stack.top (σ[x↦value.num n]) e),
+      apply step.num
+    },
+
+    case dstep.closure {
+      assume s,
+      assume h2,
+      cases h2,
+
+      existsi (stack.top (σ[f↦value.func f x R S e₁ σ]) e₂),
+      apply step.closure,
+      from spec.term value.true
+    },
+
+    case dstep.unop {
+      assume s,
+      assume h2,
+      cases h2,
+
+      existsi (stack.top (σ[y↦v]) e),
+      apply step.unop a a_1
+    },
+
+    case dstep.binop {
+      assume s,
+      assume h2,
+      cases h2,
+
+      existsi (stack.top (σ[z↦v]) e),
+      apply step.binop a a_1 a_2
+    },
+
+    case dstep.app {
+      assume s,
+      assume h2,
+      cases h2,
+
+      existsi (stack.cons ((σ'[g↦value.func g z R S e σ'][z↦v]), e) σ y f x e'),
+      apply step.app a a_1
+    },
+
+    case dstep.ite_true {
+      assume s,
+      assume h2,
+      cases h2,
+
+      existsi (stack.top σ e₁),
+      apply step.ite_true a
+    },
+
+    case dstep.ite_false {
+      assume s,
+      assume h2,
+      cases h2,
+
+      existsi (stack.top σ e₂),
+      apply step.ite_false a
+    },
+
+    case dstep.ctx d₁ d₂ R σ₁ f x y e₁ steps ih {
+      assume s,
+      assume h2,
+      cases h2,
+
+      have h3, from ih s' a,
+      cases h3 with s'' h4,
+
+      existsi (stack.cons s'' σ₁ y f x e₁),
+      apply step.ctx h4
+    },
+
+    case dstep.return {
+      assume s,
+      assume h2,
+      cases h2,
+
+      existsi (stack.top (σ₂[y↦v]) e'),
+      cases a_3,
+      apply step.return a a_1 a_2
+    }
+  end
+
+lemma step_dstep_preservation {s: stack}:
+      ∀{s': stack} {d d': dstack},
+      stack_equiv_dstack s d → (s ⟶ s') → (d ⟹ d') → stack_equiv_dstack s' d' :=
+  begin
+    induction s,
+
+    case stack.top σ e {
+      assume s' d d',
+      assume h1,
+      assume h2,
+      assume h3,
+      cases h1,
+      have h4: (dstack.top R σ e ⟹ d'), from h3,
+      cases h2,
+
+      case step.tru {
+        cases h4,
+        simp,
+        apply stack_equiv_dstack.top
+      },
+
+      case step.fals {
+        cases h4,
+        simp,
+        apply stack_equiv_dstack.top
+      },
+
+      case step.num {
+        cases h4,
+        simp,
+        apply stack_equiv_dstack.top
+      },
+
+      case step.closure {
+        cases h4,
+        simp,
+        apply stack_equiv_dstack.top
+      },
+
+      case step.unop {
+        cases h4,
+        simp,
+        have h5, from eq.trans a.symm a_2,
+        have h6: (v₁ = v₁_1), from option.some.inj h5,
+        rw[h6] at a_1,
+        have h7, from eq.trans a_1.symm a_3,
+        have h8: (v = v_1), from option.some.inj h7,
+        rw[h8],
+        apply stack_equiv_dstack.top
+      },
+
+      case step.binop {
+        cases h4,
+        simp,
+        have h5, from eq.trans a.symm a_3,
+        have h6: (v₁ = v₁_1), from option.some.inj h5,
+        rw[h6] at a_2,
+        have h7, from eq.trans a_1.symm a_4,
+        have h8: (v₂ = v₂_1), from option.some.inj h7,
+        rw[h8] at a_2,
+        have h9, from eq.trans a_2.symm a_5,
+        have h10: (v = v_1), from option.some.inj h9,
+        rw[h10],
+
+        apply stack_equiv_dstack.top
+      },
+
+      case step.app {
+        cases h4,
+        apply stack_equiv_dstack.cons,
+        have h5, from eq.trans a.symm a_2,
+        have h6: ((value.func g z R_1 S e_1 σ') = (value.func g_1 z_1 R_2 S_1 e σ'_1)),
+        from option.some.inj h5,
+        injection h6,
+        rw[h_1],
+        rw[h_2],
+        rw[h_3],
+        rw[h_4],
+        rw[h_5],
+        rw[h_6],
+        have h7, from eq.trans a_1.symm a_3,
+        have h8: (v = v_1), from option.some.inj h7,
+        rw[h8],
+        apply stack_equiv_dstack.top
+      },
+
+      case step.ite_true {
+        cases h4,
+        simp,
+        apply stack_equiv_dstack.top,
+        have h7, from eq.trans a.symm a_1,
+        have h8: (value.true = value.false), from option.some.inj h7,
+        contradiction
+      },
+
+      case step.ite_false {
+        cases h4,
+        simp,
+        have h7, from eq.trans a.symm a_1,
+        have h8: (value.false = value.true), from option.some.inj h7,
+        contradiction,
+        apply stack_equiv_dstack.top,
+      },
+    },
+
+    case stack.cons s'' σ'' f x y e'' ih {
+      assume s' d d',
+      assume h1,
+      assume h2,
+      assume h3,
+      cases h1,
+      cases h2,
+
+      case step.ctx {
+        cases h3,
+
+        apply stack_equiv_dstack.cons,
+        from ih a a_1 a_2,
+
+        simp at a,
+        cases a,
+        cases a_1
+      },
+
+      case step.return {
+        cases h3,
+
+        simp at a,
+        cases a,
+        cases a_4,
+
+        simp,
+        cases a,
+        have h5, from eq.trans a_1.symm a_4,
+        have h6: (v = v_1), from option.some.inj h5,
+        rw[h6],
+        apply stack_equiv_dstack.top,
+      }
+    }
+  end
+
+lemma step_of_dstep_trans {d d': dstack}:
+      (d ⟹* d') → ∀s, stack_equiv_dstack s d → ∃s', (s ⟶* s') ∧ stack_equiv_dstack s' d' :=
+  begin
+    assume h1,
+
+    induction h1,
+
+    assume s,
+    assume h2,
+    existsi s,
+    split,
+    from trans_step.rfl,
+    from h2,
+
+    assume s_1,
+    assume h2,
+    have h3, from ih_1 s_1 h2,
+    cases h3 with s_2 h4,
+
+
+    have h5, from step_dstep_progress.inv a_1 s_2 h4.right,
+    cases h5 with s3 h6,
+
+    existsi s3,
+    split,
+    apply trans_step.trans,
+    from h4.left,
+    from h6,
+
+    apply step_dstep_preservation h4.right h6 a_1
+  end
+
+lemma dstep_of_step_trans {s s': stack}:
+      (s ⟶* s') → ∀d, stack_equiv_dstack s d → ∃d', (d ⟹* d') ∧ stack_equiv_dstack s' d' :=
+  begin
+    assume h1,
+
+    induction h1,
+
+    assume d,
+    assume h2,
+    existsi d,
+    split,
+    from trans_dstep.rfl,
+    from h2,
+
+    assume s_1,
+    assume h2,
+    have h3, from ih_1 s_1 h2,
+    cases h3 with s_2 h4,
+
+
+    have h5: ∃ (d' : dstack), s_2⟹d', from step_dstep_progress a_1 s_2 h4.right,
+    cases h5 with s3 h6,
+
+    existsi s3,
+    split,
+    apply trans_dstep.trans,
+    from h4.left,
+    from h6,
+
+    apply step_dstep_preservation h4.right a_1 h6 
+  end
+
+lemma step_of_dstep {R₁ R₂: spec} {σ₁ σ₂: env} {e₁ e₂: exp}: (R₁, σ₁, e₁) ⟹* (R₂, σ₂, e₂) → ((σ₁, e₁) ⟶* (σ₂, e₂)) :=
+  begin
+    assume h1,
+    have h2: stack_equiv_dstack (σ₁, e₁) (R₁, σ₁, e₁), from stack_equiv_dstack.top,
+    have h3, from step_of_dstep_trans h1 (σ₁, e₁) h2,
+    cases h3 with s' h4,
+    cases h4.right,
+    from h4.left
+  end
+
+lemma value_or_step_of_dvalue_or_dstep {s: stack} {d: dstack}:
+  stack_equiv_dstack s d → (is_dvalue d ∨ ∃d', d ⟹ d') → (is_value s ∨ ∃s', s ⟶ s') :=
+  begin
+    assume h1,
+    assume h2,
+    cases h2 with h3 h3,
+    unfold is_dvalue at h3,
+    cases h3 with R h4,
+    cases h4 with σ h5,
+    cases h5 with x h6,
+    cases h6 with v h7,
+    left,
+    unfold is_value,
+    existsi σ,
+    existsi x,
+    existsi v,
+    split,
+    rw[h7.left] at h1,
+    cases h1,
+    congr,
+    from h7.right,
+    cases h3 with d' h4,
+    have h5, from step_dstep_progress.inv h4 s h1,
+    right,
+    from h5
   end
