src/theorems.lean
@@ -1,0 +1,17 @@
+import .definitions2 .qi .soundness
+
+-- This theorem states that any proposition `P` that is valid with instantiations `⟪ P ⟫` 
+-- is also a valid proposition without quantifier instantiation `⦃ P ⦄`:
+theorem vc_valid_without_instantiations (P: prop):
+  ⟪ P ⟫ → ⦃ P ⦄
+
+  := @vc_valid_from_inst_valid P -- actual proof in qi.lean
+
+
+-- This theorem states that a verified source program `e` does not get stuck,
+-- i.e. its evaluation always results either in a value or in a runtime stack `s` that can be
+-- further evaluated. The proof internally uses lemmas for progress and preservation.
+theorem verification_safety (e: exp) (s: stack) (Q: propctx):
+  (value.true ⊢ e: Q) → ((env.empty, e) ⟶* s) → (is_value s ∨ ∃s', s ⟶ s')
+  
+  := @soundness_source_programs e s Q -- actual proof in soundness.lean
