README.md
@@ -23,6 +23,11 @@ The definitions and proofs are written in [LEAN](http://leanprover.github.io/).
 - Axiomatization of SMT Logic
 - Verification of program expressions
 
+[`src/theorems.lean`](src/theorems.lean)
+
+- Quantifier Instantiation Soundness Theorem
+- Verification Safety/Soundness Theorem
+
 ## Proved Theorems
 
 **Quantifier Instantiation**
@@ -30,30 +35,31 @@ The definitions and proofs are written in [LEAN](http://leanprover.github.io/).
 Verification conditions are processed with a deterministic quantifier instantiation algorithm
 in order to ensure that checking of verification conditions is deterministic and decidable.
 
-The file [`src/qi.lean`](src/qi.lean) proves that any proposition `P` that is valid with instantiations
-`⟪ P ⟫` is also a valid proposition without quantifier instantiation `⦃ P ⦄`:
+The file [`src/theorems.lean`](src/theorems.lean) proves that
+any proposition `P` that is valid with instantiations `⟪ P ⟫`
+is also a valid proposition without quantifier instantiation `⦃ P ⦄`:
 
 ```
 ⟪ P ⟫ → ⦃ P ⦄
 ```
 
-The converse is not true. There are valid propositions that cannot be confirmed when the
+(The converse is not true. There are valid propositions that cannot be confirmed when the
 quantifier instantiation algorithm is used. Instead of relying on heuristics, the instantiation
-uses function calls in the source program as triggers.
+uses function calls in the source program as triggers.)
 
 **Verification Safety**
 
-The file [`src/soundness.lean`](src/soundness.lean) proves that a verified source program `e` does not
+The file [`src/theorems.lean`](src/theorems.lean) proves that a verified source program `e` does not
 get stuck, i.e. its evaluation always results either in a value or in a runtime stack `s` that can be
-further evaluated.
+further evaluated. The proof internally uses lemmas for progress and preservation.
 
 ```
-(true ⊢ e: Q) → ((env.empty, e) ⟶* s) → (is_value s ∨ ∃s', s ⟶ s')
+(value.true ⊢ e: Q) → ((env.empty, e) ⟶* s) → (is_value s ∨ ∃s', s ⟶ s')
 ```
 
 ## Checking the proof
 
-Assuming LEAN is installed, the proof can be checked by either building the entire package:
+Assuming LEAN is installed, the proofs can be checked by building the entire project:
 
 ```
 $ leanpkg build
@@ -62,6 +68,5 @@ $ leanpkg build
 Alternatively, is it possible to specifically check certain files, e.g.
 
 ```
-$ lean src/qi.lean
-$ lean src/soundness.lean
+$ lean src/theorems.lean
 ```
